VeriTile/Triton/DSL/Syntax.lean
@@ -144,6 +144,13 @@ syntax:70 tritonExpr:70 " % " tritonExpr:71 : tritonExpr
 syntax ident " := " tritonExpr : tritonStmt
 syntax "tl.store(" tritonExpr ", " tritonExpr ("," tritonMemKwarg)* ")" : tritonStmt
 syntax "tl.atomic_add(" tritonExpr ", " tritonExpr ("," tritonMemKwarg)* ")" : tritonStmt
+syntax "tl.atomic_max(" tritonExpr ", " tritonExpr ("," tritonMemKwarg)* ")" : tritonStmt
+syntax "tl.atomic_min(" tritonExpr ", " tritonExpr ("," tritonMemKwarg)* ")" : tritonStmt
+syntax "tl.atomic_and(" tritonExpr ", " tritonExpr ("," tritonMemKwarg)* ")" : tritonStmt
+syntax "tl.atomic_or(" tritonExpr ", " tritonExpr ("," tritonMemKwarg)* ")" : tritonStmt
+syntax "tl.atomic_xor(" tritonExpr ", " tritonExpr ("," tritonMemKwarg)* ")" : tritonStmt
+syntax "tl.atomic_xchg(" tritonExpr ", " tritonExpr ("," tritonMemKwarg)* ")" : tritonStmt
+syntax "tl.atomic_cas(" tritonExpr ", " tritonExpr ", " tritonExpr ("," tritonMemKwarg)* ")" : tritonStmt
 syntax "tl.async_copy(" tritonExpr ", " tritonExpr ("," tritonMemKwarg)* ")" : tritonStmt
 syntax "tl.async_wait()" : tritonStmt
 syntax "tl.debug_barrier()" : tritonStmt
